tests/lean/run/resolve_name_bug.lean
@@ -14,9 +14,7 @@ def g (a : nat) := a + 1
 
 example : g 0 = 1 :=
 begin
-  unfold g,
-  (target >>= check_expr ``(0 + 1 = 1)),
-  reflexivity
+  unfold g
 end
 
 example : f (f 0) = 2 :=
