tests/lean/run/unfold_issue.lean
@@ -7,7 +7,5 @@ do e ← tactic.to_expr p, guard (t = e)
 
 example (n : nat): f (n+1) n = n + 1 :=
 begin
-  unfold f,
-  (tactic.target >>= check_expr ```((n + 1 = n + 1))),
-  reflexivity,
+  unfold f
 end
